[minor] merging stronger attacker to master

cfi/abstract.v
@@ -6,6 +6,7 @@ Require Import lib.utils lib.partial_maps.
 Require Import common.common.
 Require Import lib.Coqlib.
 Require Import cfi.property.
+Require lib.list_utils.
 Set Implicit Arguments.
 
 Import ListNotations.
@@ -121,12 +122,11 @@ Inductive step : state -> state -> Prop :=
                       (State imem dmem' reg' pc' true).
 
 Inductive step_a : state -> state -> Prop :=
-| step_attack : forall imem dmem dmem' reg reg' pc i
-             (FETCH: get imem pc = Some i)
+| step_attack : forall imem dmem dmem' reg reg' pc b
              (MSAME: same_domain dmem dmem')
              (RSAME: same_domain reg reg'),
-             step_a (State imem dmem reg pc true) 
-                    (State imem dmem' reg' pc true).
+             step_a (State imem dmem reg pc b) 
+                    (State imem dmem' reg' pc b).
 
 (* Extending valid_jmp to a complete allowed CFG *)
 Definition succ (st : state) (st' : state) : bool :=
@@ -156,20 +156,16 @@ Definition succ (st : state) (st' : state) : bool :=
       end
   end.
 
-(* CH: TODO: I'm expecting the cont bit to be initially true *)
 Definition initial (s : state) := 
   cont s = true.
 
-Definition stopping (xs : list state) : Prop :=
-  exists s, xs = [s] /\ ~ exists s', step s s'.
-
 Definition all_attacker (xs : list state) : Prop :=
-  forall x1 x2, In2 x1 x2 xs -> step_a x1 x2 /\ ~step x1 x2. 
+  forall x1 x2, In2 x1 x2 xs -> step_a x1 x2.
 
 Definition all_stuck (xs : list state) : Prop :=
   forall x, In x xs -> ~ exists s, step x s.
 
-Definition stopping' (xs : list state) : Prop :=
+Definition stopping (xs : list state) : Prop :=
   all_attacker xs /\ all_stuck xs.
 
 Program Instance abstract_cfi_machine : cfi_machine := {|
@@ -183,11 +179,10 @@ Program Instance abstract_cfi_machine : cfi_machine := {|
   stopping := stopping
  |}.
 
-
 Lemma step_succ_violation ast ast' :
    succ ast ast' = false ->
    step ast ast' ->
-   cont ast' = false.
+   cont ast = true /\ cont ast' = false. 
 Proof.
   intros SUCC STEP.
   inversion STEP; subst; simpl in SUCC; rewrite FETCH in SUCC;
@@ -201,15 +196,87 @@ Qed.
 
 Lemma step_a_violation ast ast' :
    step_a ast ast' ->
-   cont ast = true.
+   cont ast = cont ast'.
 Proof.
   intros STEP.
   inversion STEP; subst. reflexivity.
 Qed.
 
+Lemma list_theorem {X} (x : X) xs hs y z tl x0 :
+  xs ++ [x] = hs ++ y :: z :: tl ++ [x0] ->
+  x = x0.
+Proof.
+  intro H.
+  gdep hs. gdep y. gdep z. gdep tl.
+  induction xs.
+  - intros. simpl in H. repeat (destruct hs; inversion H).
+  - intros. destruct hs.
+    + simpl in H. inversion H. subst.
+      destruct tl.
+      * simpl in *.
+        destruct xs; simpl in H2; [inversion H2 | idtac].
+        destruct xs; simpl in *.
+        inv H2. reflexivity.
+        destruct xs; simpl in H2; inversion H2.
+      * simpl in H2.
+        specialize (IHxs tl x1 z []). apply IHxs.
+        auto.
+    + inv H.
+      eapply IHxs; eauto.
+Qed.
+
+
+
+Lemma all_attacker_red ast ast' axs :
+  all_attacker (ast :: ast' :: axs) ->
+  all_attacker (ast' :: axs).
+Proof.
+  intros ATTACKER asi asj IN2.
+  assert (IN2' : In2 asi asj (ast :: ast' :: axs))
+    by (simpl; auto).
+  apply ATTACKER in IN2'.
+  assumption.
+Qed.
+
+Lemma all_stuck_red ast ast' axs :
+  all_stuck (ast :: ast' :: axs) ->
+  all_stuck (ast' :: axs).
+Proof.
+  intros ALLS asi IN.
+  unfold all_stuck in ALLS.
+  assert (IN': In asi (ast :: ast' :: axs))
+    by (simpl; right; auto).
+  auto.
+Qed.
+  
+Lemma stuck_states_preserved_by_a asi tl :
+  all_attacker (asi :: tl) ->
+  cont asi = false ->
+  forall asj, In asj tl -> cont asj = false.
+Proof.
+  intros ALLATTACKER CONT asj IN.
+  gdep asi.
+  induction tl; intros.
+  - destruct IN.
+  - destruct IN as [? | IN].
+    + subst. 
+      assert (IN2: In2 asi asj (asi :: asj :: tl))
+        by (simpl; auto).
+      apply ALLATTACKER in IN2.
+      destruct (step_a_violation IN2).
+      assumption.
+    + assert (IN2: In2 asi a (asi :: a :: tl))
+        by (simpl; auto).
+      apply ALLATTACKER in IN2.
+      assert (CONT' := step_a_violation IN2).
+      rewrite CONT' in CONT.
+      apply all_attacker_red in ALLATTACKER.
+      eapply IHtl; eauto.
+Qed.
+
 Theorem cfi : cfi abstract_cfi_machine.
 Proof.
-  unfold cfi. intros.
+ unfold cfi. intros.
   apply interm_equiv_intermrev in INTERM.
   induction INTERM as [s s' STEP | s s' s'' xs STEP INTERM ].
   + destruct (succ s s') eqn:SUCC.
@@ -220,20 +287,23 @@ Proof.
     * (*case the step is outside the contro flow graph*)
       destruct STEP as [STEPA | STEP].
       - (*case it's an attacker step*)
-        left. intros si sj IN2.
+        left. intros si sj IN2. simpl in *.
         destruct IN2 as [[? ?] | CONTRA]; [subst | destruct CONTRA].
-        auto.
-        intro STEP. assert (CONTRA := step_succ_violation SUCC STEP).
-        inversion STEPA. subst. discriminate.
+        intro STEP.
+        destruct (step_succ_violation SUCC STEP) as [CONT1 CONT2].
+        assert (CONTRA := step_a_violation STEPA).
+        rewrite CONTRA in CONT1. congruence.
       - (*case it's a normal step*)
         right; exists s; exists s'; exists []; exists [].
         simpl; repeat (split;auto).
         intros ? ? IN2. destruct IN2.
         intros ? ? IN2. destruct IN2.
-        unfold stopping. exists s'. split; auto.
-        intro CONTRA. destruct CONTRA as [s'' CONTRA].
-        assert (FLAG := step_succ_violation SUCC STEP).
-        inv CONTRA; simpl in FLAG; discriminate.
+        unfold stopping. 
+        intros si sj CONTRA. by destruct CONTRA.
+        intros si IN. destruct IN as [? | IN]; [subst | destruct IN].
+        destruct (step_succ_violation SUCC STEP) as [H1 H2].
+        intros (? & CONTRA).
+        inv CONTRA; simpl in H2; by discriminate.     
   + apply interm_equiv_intermrev in INTERM.
     destruct (IHINTERM INIT) as [TSAFE | [sv1 [sv2 [hs [tl VIOLATION]]]]].
     { unfold trace_has_cfi in TSAFE.
@@ -261,8 +331,9 @@ Proof.
           destruct (in2_reverse IN2) as [IN2' | [EQ1 EQ2]].
           - apply TSAFE; assumption.
           - subst. apply interm_last_step in INTERM; subst; auto.
-            intro STEP. assert (CONTRA := step_succ_violation SUCC STEP).
-            inversion STEPA; subst; discriminate. }
+            intro STEP. destruct (step_succ_violation SUCC STEP) as [H1 H2].
+            assert (CONTRA := step_a_violation STEPA).
+            rewrite CONTRA in H1. congruence. }
       - (*case it's a normal step*)
         right. induction xs using rev_ind; [inversion INTERM | idtac].
         apply interm_last_step in INTERM; subst.
@@ -270,26 +341,224 @@ Proof.
         simpl; rewrite <- app_assoc. repeat (split; auto).
         intros ? ? IN2.
         destruct IN2.
-        unfold stopping. exists s''. split; [reflexivity | idtac].
-        intro CONTRA. destruct CONTRA as [s''' CONTRA].
-        assert (FLAG := step_succ_violation SUCC STEP).
-        inv CONTRA; simpl in FLAG; discriminate.
+        unfold stopping. 
+        intros ? ? CONTRA. destruct CONTRA.
+        intros si IN.
+        destruct IN as [? | IN]; [subst | destruct IN].
+        destruct (step_succ_violation SUCC STEP) as [H1 H2].
+        intros (? & CONTRA).
+        inv CONTRA; simpl in H2; by discriminate.   
     }
-    { (*Case a violation occurs in the trace*)
+    { (*Case a violation occurs in the trace*) 
      induction xs using rev_ind; [inversion INTERM | subst; clear IHxs].
      destruct VIOLATION as [LST [VIO [T1 [T2 STOPS]]]].
-     rewrite LST in INTERM. unfold stopping in STOPS.
-     destruct STOPS as [sv2' [EQ IRRED]].
-     destruct tl; [simpl; inversion EQ; subst | inversion EQ].
-     change [sv1;sv2'] with ([sv1] ++ [sv2']) in INTERM.
-     remember (hs ++ [sv1]) as hs'.
-     rewrite app_assoc in INTERM.
-     rewrite <- Heqhs' in INTERM.
-     apply interm_last_step in INTERM; subst.
+     rewrite LST in INTERM. simpl in *.
+     destruct STOPS as [ALLATTACKER ALLSTUCK].
      destruct VIO as [VSTEP SUCC].
-     assert (FLAG := step_succ_violation SUCC VSTEP).
-     destruct STEP as [STEP | STEP];
-       inv STEP; simpl in FLAG; discriminate.
+     destruct (step_succ_violation SUCC VSTEP) as [H1 H2].
+     destruct STEP as [STEPA | STEP].
+     - unfold trace_has_at_most_one_violation.
+       right.
+       rewrite LST.
+       exists sv1; exists sv2; exists hs; exists (tl ++ [s'']).
+       split. 
+       { rewrite <- app_assoc. by reflexivity. }
+       { split. 
+         { simpl; split; by auto. }
+         { split; [assumption | simpl].
+           split.
+           - intros si sj IN2 STEP.
+             induction tl using rev_ind.
+             * simpl in IN2. 
+               destruct IN2 as [[? ?] | CONTRA]; [subst | destruct CONTRA].
+               inv STEP; simpl in H2; discriminate.
+             * clear IHtl.
+               rewrite <- LST in INTERM.
+               assert (EQ := list_theorem x xs hs sv1 sv2 tl x0 LST).
+               subst.
+               apply interm_last_step in INTERM; subst.
+               rewrite <- app_assoc in IN2.
+               simpl ((sv2 :: tl ++ [s'] ++ [s''])) in IN2.
+               rewrite app_comm_cons in IN2.
+               remember (sv2 :: tl) as tl'.
+               destruct (in2_reverse IN2) as [IN2' | [? ?]]; subst.
+               + unfold all_stuck in ALLSTUCK.
+                 apply In2_implies_In in IN2'.
+                 apply ALLSTUCK in IN2'.
+                 assert (ESTEP: exists s, step si s)
+                   by (eexists; eauto).
+                 destruct (IN2' ESTEP).
+               + destruct (succ si sj) eqn:SUCC'.
+                 * assumption.
+                 * destruct (step_succ_violation SUCC' STEP) as [H3 H4].
+                   assert (EQ := step_a_violation STEPA).
+                   rewrite EQ in H3.
+                   congruence.
+           - unfold stopping.
+             split.
+             { (*all attacker*)
+               intros si sj IN2.
+               destruct tl using rev_ind.
+               - simpl in IN2. 
+                 destruct IN2 as [[? ?] | CONTRA]; [subst | destruct CONTRA].
+                 change (hs ++ [sv1; si]) with (hs ++ [sv1] ++ [si]) in INTERM.
+                 rewrite app_assoc in INTERM.
+                 apply interm_last_step in INTERM; subst.
+                 assumption.
+               - clear IHtl.
+                 rewrite <- LST in INTERM.
+                 apply list_theorem in LST; subst.
+                 apply interm_last_step in INTERM; subst.
+                 rewrite <- app_assoc in IN2.
+                 simpl (sv2 :: tl ++ [s'] ++ [s'']) in IN2.
+                 rewrite app_comm_cons in IN2.
+                 destruct (in2_reverse IN2) as [IN2' | [? ?]]; subst.
+                 + apply ALLATTACKER; assumption.
+                 + assumption.
+             }
+             { (*all stuck*)
+               intros si IN.
+               destruct tl using rev_ind.
+               - destruct IN as [? | IN].
+                 + subst. intros (? & CONTRA).
+                   destruct (step_succ_violation SUCC VSTEP) as [H3 H4].
+                   inv CONTRA; simpl in H3; by discriminate.  
+                 + destruct IN as [? | CONTRA].
+                   * subst. intros (? & CONTRA).
+                     destruct (step_succ_violation SUCC VSTEP) as [H3 H4].
+                     change (hs ++ [sv1;sv2]) with (hs ++ [sv1] ++ [sv2]) in INTERM.
+                     rewrite app_assoc in INTERM.
+                     apply interm_last_step in INTERM. subst.
+                     assert (EQ:= step_a_violation STEPA).
+                     rewrite EQ in H4.
+                     inv CONTRA; simpl in H4; by discriminate. 
+                   * destruct CONTRA.
+               - clear IHtl.
+                 rewrite app_comm_cons in IN.
+                 apply list_utils.in_reverse in IN.
+                 destruct IN as [IN | ?]; subst.
+                 + apply ALLSTUCK; by assumption.
+                 + rewrite <- LST in INTERM.
+                   assert (EQ:= interm_last_step INTERM); 
+                   apply list_theorem in LST; subst.
+                   subst.
+                   unfold all_stuck in ALLSTUCK.
+                   specialize (ALLSTUCK s').
+                   assert (IN: In s' (sv2 :: tl ++ [s']))
+                     by (eauto using list_utils.in_last).
+                   assert (STUCK := stuck_states_preserved_by_a ALLATTACKER H2).
+                   assert (IN' : In s' (tl ++ [s']))
+                     by (eauto using list_utils.in_last).
+                   apply STUCK in IN'.
+                   assert (CONT := step_a_violation STEPA).
+                   rewrite CONT in IN'.
+                   intros (? & CONTRA).
+                   inv CONTRA; simpl in IN'; discriminate.
+             }
+         }
+       }
+     - right.
+       rewrite LST.
+       exists sv1; exists sv2; exists hs; exists (tl ++ [s'']).
+       split. 
+       { rewrite <- app_assoc. by reflexivity. }
+       { split. 
+         { simpl; split; by auto. }
+         { split; [assumption | simpl].
+           split.
+           - intros si sj IN2 STEP'.
+             induction tl using rev_ind.
+             * simpl in IN2. 
+               destruct IN2 as [[? ?] | CONTRA]; [subst | destruct CONTRA].
+               inv STEP'; simpl in H2; discriminate.
+             * clear IHtl.
+               rewrite <- LST in INTERM.
+               assert (EQ := list_theorem x xs hs sv1 sv2 tl x0 LST).
+               subst.
+               apply interm_last_step in INTERM; subst.
+               rewrite <- app_assoc in IN2.
+               simpl ((sv2 :: tl ++ [s'] ++ [s''])) in IN2.
+               rewrite app_comm_cons in IN2.
+               remember (sv2 :: tl) as tl'.
+               destruct (in2_reverse IN2) as [IN2' | [? ?]]; subst.
+               + unfold all_stuck in ALLSTUCK.
+                 apply In2_implies_In in IN2'.
+                 apply ALLSTUCK in IN2'.
+                 assert (ESTEP: exists s, step si s)
+                   by (eexists; eauto).
+                 destruct (IN2' ESTEP).
+               + unfold all_stuck in ALLSTUCK.
+                 assert (IN: In si (sv2 :: tl ++ [si]))
+                   by (eauto using list_utils.in_last).
+                 apply ALLSTUCK in IN.
+                 assert (ESTEP : exists s, step si s) 
+                   by (eexists; eauto).
+                 destruct (IN ESTEP).
+           - unfold stopping.
+             split.
+             { (*all attacker*)
+               intros si sj IN2.
+               destruct tl using rev_ind.
+               - simpl in IN2. 
+                 destruct IN2 as [[? ?] | CONTRA]; [subst | destruct CONTRA].
+                 change (hs ++ [sv1; si]) with (hs ++ [sv1] ++ [si]) in INTERM.
+                 rewrite app_assoc in INTERM.
+                 apply interm_last_step in INTERM; subst.
+                 assert (IN: In s' [s']) by (simpl; auto).
+                 apply ALLSTUCK in IN.
+                 exfalso.
+                 apply IN. eexists; eauto.
+               - clear IHtl.
+                 rewrite <- LST in INTERM.
+                 apply list_theorem in LST; subst.
+                 apply interm_last_step in INTERM; subst.
+                 rewrite <- app_assoc in IN2.
+                 simpl (sv2 :: tl ++ [s'] ++ [s'']) in IN2.
+                 rewrite app_comm_cons in IN2.
+                 destruct (in2_reverse IN2) as [IN2' | [? ?]]; subst.
+                 + apply ALLATTACKER; assumption.
+                 + assert (IN: In si (sv2 :: tl ++ [si]))
+                     by (eauto using list_utils.in_last).
+                   apply ALLSTUCK in IN.
+                   exfalso. apply IN. eexists; eauto.
+             }
+             { (*all stuck*)
+               intros si IN.
+               destruct tl using rev_ind.
+               - destruct IN as [? | IN].
+                 + subst. intros (? & CONTRA).
+                   destruct (step_succ_violation SUCC VSTEP) as [H3 H4].
+                   inv CONTRA; simpl in H3; by discriminate.  
+                 + destruct IN as [? | CONTRA].
+                   * subst. intros (? & CONTRA).
+                     destruct (step_succ_violation SUCC VSTEP) as [H3 H4].
+                     change (hs ++ [sv1;sv2]) with (hs ++ [sv1] ++ [sv2]) in INTERM.
+                     rewrite app_assoc in INTERM.
+                     apply interm_last_step in INTERM. subst.
+                     assert (IN: In s' [s']) by (simpl; auto).
+                     apply ALLSTUCK in IN.
+                     exfalso.
+                     apply IN. eexists; eauto. 
+                   * destruct CONTRA.
+               - clear IHtl.
+                 rewrite app_comm_cons in IN.
+                 apply list_utils.in_reverse in IN.
+                 destruct IN as [IN | ?]; subst.
+                 + apply ALLSTUCK; by assumption.
+                 + rewrite <- LST in INTERM.
+                   assert (EQ:= interm_last_step INTERM); 
+                   apply list_theorem in LST; subst.
+                   subst.
+                   unfold all_stuck in ALLSTUCK.
+                   specialize (ALLSTUCK s').
+                   assert (IN: In s' (sv2 :: tl ++ [s']))
+                     by (eauto using list_utils.in_last).
+                  apply ALLSTUCK in IN.
+                  exfalso.
+                  apply IN; eexists; eauto.
+             }
+         }
+       }           
     }
 Qed.
 
